cv_translator/backend_arm8_cvScript.sml
@@ -242,14 +242,18 @@ QED
 val _ = cv_trans word_to_word_inlogic_arm8_def;
 val _ = cv_trans from_word_0_arm8_def;
 
-val _ = compile_0_arm8_def
-  |> SRULE [data_to_wordTheory.stubs_def,backend_64_cvTheory.inline]
-  |> cv_auto_trans;
+val _ = cv_trans (compile_0_arm8_def
+                    |> SRULE [data_to_wordTheory.stubs_def,
+                              backend_64_cvTheory.inline,
+                              to_map_compile_part]);
 
-(*
-backend_arm8Theory.to_word_0_arm8_def
-backend_arm8Theory.compile_cake_arm8_def
-*)
+val _ = cv_trans backend_arm8Theory.to_word_0_arm8_def;
+val _ = cv_auto_trans backend_arm8Theory.to_livesets_0_arm8_def;
+
+(* main two translations below *)
+
+val _ = cv_trans backend_arm8Theory.to_livesets_arm8_def;
+val _ = cv_trans backend_arm8Theory.compile_cake_arm8_def;
 
 val _ = Feedback.set_trace "TheoryPP.include_docs" 0;
 val _ = export_theory();
